libcrux-ml-kem/proofs/fstar/extraction/Libcrux_ml_kem.Polynomial.fst
@@ -348,7 +348,7 @@ let poly_barrett_reduce
   in
   myself
 
-#push-options "--admit_smt_queries true"
+#push-options "--z3rlimit 300"
 
 let subtract_reduce
       (#v_Vector: Type0)
@@ -357,43 +357,81 @@ let subtract_reduce
           Libcrux_ml_kem.Vector.Traits.t_Operations v_Vector)
       (myself b: t_PolynomialRingElement v_Vector)
      =
+  let e_b:t_Array v_Vector (mk_usize 16) = b.f_coefficients in
   let b:t_PolynomialRingElement v_Vector =
     Rust_primitives.Hax.Folds.fold_range (mk_usize 0)
       v_VECTORS_IN_RING_ELEMENT
-      (fun b temp_1_ ->
+      (fun b i ->
           let b:t_PolynomialRingElement v_Vector = b in
-          let _:usize = temp_1_ in
-          true)
+          let i:usize = i in
+          (forall j. j < v i ==> is_bounded_vector 3328 b.f_coefficients.[ sz j ]) /\
+          (forall j. (j >= v i /\ j < 16) ==> b.f_coefficients.[ sz j ] == e_b.[ sz j ]))
       b
       (fun b i ->
           let b:t_PolynomialRingElement v_Vector = b in
           let i:usize = i in
+          let _:Prims.unit =
+            assert (v i < 16);
+            assert_norm (1441 < pow2 15);
+            assert_norm (1664 < pow2 15);
+            assert_norm (mk_i16 1441 <. mk_i16 1664);
+            assert (Spec.Utils.is_i16b 1664 (mk_i16 1441))
+          in
           let coefficient_normal_form:v_Vector =
             Libcrux_ml_kem.Vector.Traits.f_montgomery_multiply_by_constant #v_Vector
               #FStar.Tactics.Typeclasses.solve
               (b.f_coefficients.[ i ] <: v_Vector)
               (mk_i16 1441)
           in
+          let _:Prims.unit =
+            assert (is_bounded_vector 3328 coefficient_normal_form);
+            assert (is_bounded_vector (pow2 12 - 1) (myself.f_coefficients.[ i ]));
+            assert_norm (pow2 12 - 1 == 4095);
+            Spec.Utils.lemma_sub_intb_forall 4095 3328;
+            assert (forall j.
+                  Spec.Utils.is_intb 7423
+                    (v (Seq.index (i1.f_to_i16_array myself.f_coefficients.[ i ]) j) -
+                      v (Seq.index (i1.f_to_i16_array coefficient_normal_form) j)));
+            assert_norm (7423 <= pow2 15 - 1);
+            Spec.Utils.lemma_intb_le 7423 (pow2 15 - 1);
+            Spec.Utils.lemma_intb_le 7423 28296;
+            assert (forall j.
+                  Spec.Utils.is_intb (pow2 15 - 1)
+                    (v (Seq.index (i1.f_to_i16_array myself.f_coefficients.[ i ]) j) -
+                      v (Seq.index (i1.f_to_i16_array coefficient_normal_form) j)));
+            assert (forall j.
+                  Spec.Utils.is_intb 28296
+                    (v (Seq.index (i1.f_to_i16_array myself.f_coefficients.[ i ]) j) -
+                      v (Seq.index (i1.f_to_i16_array coefficient_normal_form) j)))
+          in
+          let diff:v_Vector =
+            Libcrux_ml_kem.Vector.Traits.f_sub #v_Vector
+              #FStar.Tactics.Typeclasses.solve
+              (myself.f_coefficients.[ i ] <: v_Vector)
+              coefficient_normal_form
+          in
+          let _:Prims.unit = assert (is_bounded_vector 28296 diff) in
+          let red:v_Vector =
+            Libcrux_ml_kem.Vector.Traits.f_barrett_reduce #v_Vector
+              #FStar.Tactics.Typeclasses.solve
+              diff
+          in
+          let _:Prims.unit = assert (is_bounded_vector 3328 red) in
           let b:t_PolynomialRingElement v_Vector =
             {
               b with
               f_coefficients
               =
-              Rust_primitives.Hax.Monomorphized_update_at.update_at_usize b.f_coefficients
-                i
-                (Libcrux_ml_kem.Vector.Traits.f_barrett_reduce #v_Vector
-                    #FStar.Tactics.Typeclasses.solve
-                    (Libcrux_ml_kem.Vector.Traits.f_sub #v_Vector
-                        #FStar.Tactics.Typeclasses.solve
-                        (myself.f_coefficients.[ i ] <: v_Vector)
-                        coefficient_normal_form
-                      <:
-                      v_Vector)
-                  <:
-                  v_Vector)
+              Rust_primitives.Hax.Monomorphized_update_at.update_at_usize b.f_coefficients i red
             }
             <:
             t_PolynomialRingElement v_Vector
+          in
+          let _:Prims.unit =
+            assert (forall j. (j > v i /\ j < 16) ==> b.f_coefficients.[ sz j ] == e_b.[ sz j ]);
+            assert (forall j. j < v i ==> is_bounded_vector 3328 b.f_coefficients.[ sz j ]);
+            assert (b.f_coefficients.[ i ] == red);
+            assert (forall j. j <= v i ==> is_bounded_vector 3328 b.f_coefficients.[ sz j ])
           in
           b)
   in
@@ -670,14 +708,6 @@ let impl_2__ZERO
   <:
   t_PolynomialRingElement v_Vector
 
-let impl_2__subtract_reduce
-      (#v_Vector: Type0)
-      (#[FStar.Tactics.Typeclasses.tcresolve ()]
-          i1:
-          Libcrux_ml_kem.Vector.Traits.t_Operations v_Vector)
-      (self b: t_PolynomialRingElement v_Vector)
-     = subtract_reduce #v_Vector self b
-
 let impl_2__add_message_error_reduce
       (#v_Vector: Type0)
       (#[FStar.Tactics.Typeclasses.tcresolve ()]
@@ -858,6 +888,14 @@ let impl_2__poly_barrett_reduce
      =
   let self:t_PolynomialRingElement v_Vector = poly_barrett_reduce #v_Vector self in
   self
+
+let impl_2__subtract_reduce
+      (#v_Vector: Type0)
+      (#[FStar.Tactics.Typeclasses.tcresolve ()]
+          i1:
+          Libcrux_ml_kem.Vector.Traits.t_Operations v_Vector)
+      (self b: t_PolynomialRingElement v_Vector)
+     = subtract_reduce #v_Vector self b
 
 let impl_2__add_standard_error_reduce
       (#v_Vector: Type0)
